theories/RTac/InContext.v
@@ -7,13 +7,24 @@ Set Implicit Arguments.
 Set Strict Implicit.
 
 Section with_instantiation.
-(*  Variable inst : Type. *)
   Variable typ expr : Type.
   Variable m : Type -> Type.
   Context {Monad_m : Monad m}.
 
   Definition InContext (ctx : Ctx typ expr) (T : Type) : Type :=
     ctx_subst ctx -> m (ctx_subst ctx * T).
+
+
+  Global Instance Monad_InContext ctx : Monad (InContext ctx) :=
+  { bind := fun _T _U c k ctx =>
+      bind (c ctx)
+           (fun ctx_r => let '(ctx',r') := ctx_r in
+                         k r' ctx')
+  ; ret := fun _T v ctx => ret (ctx, v) }.
+
+  Global Instance MonadT_InContext ctx : MonadT (InContext ctx) m :=
+  { lift := fun _T x ctx => bind x (fun x => ret (ctx, x)) }.
+
 
   Definition assume {T} (m : option T) (k : T -> Prop) : Prop :=
     match m with
@@ -27,12 +38,6 @@ Section with_instantiation.
     | Some x => k x
     end.
 
-  Variable mPred : forall {T}, (T -> Prop) -> m T -> Prop.
-
-  (* NOTE: The problem with this definition is that it leaves too much
-   * exposed.
-   * -
-   *)
   Variable RType_typ : RType typ.
   Variable Expr_expr : Expr RType_typ expr.
   Variable Typ0_Prop : Typ0 _ Prop.
@@ -48,36 +53,120 @@ Section with_instantiation.
   : exprT (getUVars c) (getVars c) T :=
     fun us vs => env (us,vs).
 
-  Definition InContext_spec (WFi : forall ctx, ctx_subst ctx -> Prop)
+  SearchAbout ctx_subst.
+
+  Let WFi := @WellFormed_ctx_subst typ expr _ _.
+
+  Require Import Morphisms.
+
+  Class MonadLogic : Type :=
+  { MLogic : Type := Prop
+  ; Mentails : MLogic -> MLogic -> Prop := fun x y => x -> y (** This should be a charge logic **)
+  ; ltrue : MLogic := True
+  ; limpl : MLogic -> MLogic -> MLogic := fun x y => x -> y
+  ; Pred : forall {T}, (T -> MLogic) -> m T -> Prop
+  ; Pred_ret : forall T (x : T) (P : T -> MLogic), Mentails ltrue (P x) -> Pred P (Monad.ret x)
+  ; Pred_bind : forall T U (c : m T) (k : T -> m U) (P : T -> MLogic) (Pu : U -> MLogic),
+      Pred P c ->
+      (forall x, Pred (fun y => limpl (P x) (Pu y)) (k x)) ->
+      Pred Pu (Monad.bind c k)
+  ; Proper_Pred : forall {T}, Proper ((pointwise_relation _ Mentails) ==> eq ==> Basics.impl)%signature (@Pred T)
+  }.
+
+  Variable (ML : MonadLogic).
+
+  Definition InContext_spec
              {T}
+             (K : Prop)
              (WFg : T -> Prop)
-             (TD : forall ctx, T -> option (env_of_Ctx ctx -> Prop))
-             (c : Ctx typ expr) (t : InContext c T) : Prop :=
-    forall (i : ctx_subst c), WFi c i ->
-    assume (pctxD i) (fun C =>
-      mPred (fun i_g => let '(i',g') := i_g in
-                        WFg g' /\ WFi c i' /\
+             (c : Ctx typ expr)
+             (TD : T -> option (env_of_Ctx c -> Prop))
+             (t : InContext c T) : Prop :=
+    forall (i : ctx_subst c),
+      Pred (fun i_g => let '(i',g') := i_g in
+                        K -> WFi i -> WFg g' /\ WFi i' /\
+                        assume (pctxD i) (fun C =>
                         assert (pctxD i') (fun I' =>
-                        assert (TD c g') (fun G' =>
-                                            SubstMorphism i i' /\
-                                            forall us vs,
-                                              I' (exprT_of_env G') us vs)))
-            (t i)).
+                        assert (TD g') (fun G' =>
+                                          SubstMorphism i i' /\
+                                          forall us vs,
+                                            I' (exprT_of_env G') us vs))))
+            (t i).
 
-(*
-  Definition lift {T} (x : m T) : InContext T :=
-    fun _ ctx => bind (m:=m) x (fun x => ret (m:=m) (ctx, x)).
-*)
+  Require Import ExtLib.Tactics.
 
-  Global Instance Monad_InContext ctx : Monad (InContext ctx) :=
-  { bind := fun _T _U c k ctx =>
-      bind (c ctx)
-           (fun ctx_r => let '(ctx',r') := ctx_r in
-                         k r' ctx')
-  ; ret := fun _T v ctx => ret (ctx, v) }.
+  Lemma InContext_spec_ret
+  : forall ctx {T} (val : T)
+           (wfGoal : _ -> Prop) (goalD : T -> option (env_of_Ctx ctx -> Prop)),
+      (forall i cD,
+          pctxD (ctx:=ctx) i = Some cD ->
+          wfGoal val /\
+          exists gD,
+            goalD val = Some gD /\
+            forall us vs, cD (fun us vs => gD (us, vs)) us vs) ->
+      InContext_spec (c:=ctx) (wfGoal val) wfGoal goalD (Monad.ret val).
+  Proof.
+    simpl. intros. red. intros.
+    specialize (H i).
+    destruct (pctxD i) eqn:Heq.
+    { simpl.
+      eapply Pred_ret.
+      red. intros.
+      specialize (H _ eq_refl).
+      forward_reason.
+      split; auto. split; eauto.
+      rewrite Heq. simpl.
+      rewrite H3. simpl. split; eauto. reflexivity. }
+    { simpl. eapply Pred_ret. red. tauto. }
+  Qed.
 
-  Global Instance MonadT_InContext ctx : MonadT (InContext ctx) m :=
-  { lift := fun _T x ctx => bind x (fun x => ret (ctx, x)) }.
+  Lemma InContext_spec_bind
+  : forall ctx {T U} (K : Prop)
+           (wfGoalT : _ -> Prop) (goalDT : T -> option (env_of_Ctx ctx -> Prop))
+           (wfGoalU : _ -> Prop) (goalDU : U -> option (env_of_Ctx ctx -> Prop))
+           (c : InContext ctx T) (k : T -> InContext ctx U),
+      InContext_spec (c:=ctx) K wfGoalT goalDT c ->
+      (forall x,
+          InContext_spec (c:=ctx) (K /\ wfGoalT x)
+                         wfGoalU
+                         (fun y => match goalDU y with
+                                   | None => None
+                                   | Some P => Some (fun e => wfGoalT x -> P e)
+                                   end) (k x)) ->
+      InContext_spec (c:=ctx) K wfGoalU goalDU (Monad.bind c k).
+  Proof.
+    simpl. intros. red. intros.
+    specialize (H i).
+    simpl in *.
+    eapply Pred_bind.
+    { eapply H. }
+    { simpl. destruct x. clear H.
+      specialize (H0 t c0).
+      revert H0.
+      eapply Proper_Pred; [ | reflexivity ].
+      { red. intros.
+        destruct a. red. unfold limpl. intros.
+        forward_reason.
+        split; auto. split; auto.
+        destruct (pctxD i) eqn:Heq; simpl in *; auto.
+        destruct (pctxD c0) eqn:Heq'; simpl in *; try contradiction.
+        destruct (pctxD c1) eqn:Heq''; simpl in *; try contradiction.
+        destruct (goalDT t); simpl in *; try contradiction.
+        destruct (goalDU u); simpl in *; try contradiction.
+        forward_reason.
+        split.
+        { etransitivity; eauto. }
+        { intros.
+          specialize (H7 us vs).
+          specialize (H8 us vs).
+          gather_facts.
+          eapply pctxD_SubstMorphism; [ | | eassumption | ]; eauto.
+          gather_facts.
+          eapply pctxD_SubstMorphism; [ | | eassumption | ]; eauto.
+          eapply Pure_pctxD; eauto.
+          unfold exprT_of_env.
+          intros; tauto. } } }
+  Qed.
 
   (** Probably do not want to expose this *)
   Definition getInst ctx : InContext ctx (ctx_subst ctx) :=
@@ -102,311 +191,9 @@ Section with_instantiation.
 
   Definition freshUVar {T} (t : typ) (c : uvar -> InContext T) : InContext T.
   Admitted.
-
-  (** TODO: This should really be with respect to an underlying exception monad *)
-  Definition unify (e1 e2 : expr) (t : typ) : InContext bool.
-  Admitted.
 *)
+
+  Definition unify ctx (e1 e2 : expr) (t : typ) : InContext ctx bool.
+  Admitted.
+
 End with_instantiation.
-
-Require Import Morphisms.
-
-(*
-Section with_error.
-  Definition Error (T : Type) : Type := option T.
-
-  Definition PredError {T} (P : T -> Prop) (m : Error T) : Prop :=
-    match m with
-    | None => True
-    | Some x => P x
-    end.
-
-  Definition Error_bind {T U} (m : Error T) (k : T -> Error U) : Error U :=
-    match m with
-    | None => None
-    | Some x => k x
-    end.
-
-  Theorem Error_bind_sound
-  : forall {T U} (P : _ -> Prop) (Q : _ -> _ -> Prop) m k,
-      PredError P m ->
-      (forall x, PredError (fun z => P x -> Q x z) (k x)) ->
-      PredError (fun z => exists x, P x /\ Q x z) (@Error_bind T U m k).
-  Proof.
-    compute. intros.
-    destruct m; auto.
-    specialize (H0 t).
-    destruct (k t); auto.
-    eauto.
-  Qed.
-
-  Theorem Error_ret_sound {T} (v : T) : PredError (eq v) (Some v).
-  Proof.
-    reflexivity.
-  Qed.
-
-End with_error.
-*)
-
-Section with_error.
-  Definition Error (T : Type) : Type := option T.
-
-  Definition PredError {T} (P : (T -> Prop) -> Prop) (m : Error T) : Prop :=
-    match m with
-    | None => True
-    | Some x => P (eq x)
-    end.
-
-  Definition Error_bind {T U} (m : Error T) (k : T -> Error U) : Error U :=
-    match m with
-    | None => None
-    | Some x => k x
-    end.
-
-  Theorem Error_bind_sound
-  : forall {T U} (P : (T -> Prop) -> Prop) (Q : _ -> Prop) m k,
-      PredError P m ->
-      (forall x, PredError (fun kP => P (eq x) -> Q kP) (k x)) ->
-      PredError Q (@Error_bind T U m k).
-  Proof.
-    compute. intros.
-    destruct m; auto.
-    specialize (H0 t).
-    destruct (k t); auto.
-  Qed.
-
-  Theorem Error_ret_sound {T} (v : T) : PredError (fun kP => kP v) (Some v).
-  Proof.
-    reflexivity.
-  Qed.
-
-  Theorem Error_fail_sound {T} : PredError (fun kP => False) (@None T).
-  Proof.
-    exact I.
-  Qed.
-
-  Theorem Proper_PredError_iff {T}
-  : Proper (((eq ==> iff) ==> iff) ==> eq ==> iff)%signature
-           (@PredError T).
-  Proof.
-    cbv beta iota zeta delta - [ iff ].
-    intros. subst.
-    destruct y0; try tauto.
-    eapply H. intros; subst; tauto.
-  Qed.
-
-  Theorem Proper_PredError_impl {T}
-  : Proper (((eq ==> iff) ==> Basics.impl) ==> eq ==> Basics.impl)%signature
-           (@PredError T).
-  Proof.
-    cbv beta iota zeta delta - [ iff ].
-    intros. subst.
-    destruct y0; try tauto.
-    revert H1. eapply H.
-    intros. subst. tauto.
-  Qed.
-
-  Opaque PredError.
-
-  Goal PredError (fun kP => kP 3) (Error_bind (Some 3) (@Some _)).
-  Proof.
-    eapply Error_bind_sound.
-    eapply Error_ret_sound.
-    simpl.
-    intros.
-    eapply Proper_PredError_impl.
-    2: reflexivity.
-    2: eapply Error_ret_sound.
-    cbv beta iota zeta delta - [ iff ].
-    intros; subst. eapply H; eauto.
-  Qed.
-
-  Goal PredError (T:=nat) (fun kP => False) (Error_bind None (@Some _)).
-  Proof.
-    eapply Error_bind_sound.
-    eapply Error_fail_sound.
-    simpl.
-    intros.
-    eapply Proper_PredError_impl.
-    2: reflexivity.
-    2: eapply Error_ret_sound.
-    cbv beta iota zeta delta - [ iff ].
-    intros; subst.
-    inversion H1.
-  Qed.
-
-End with_error.
-
-(*
-Section with_error.
-  Definition Error (T : Type) : Type :=
-    forall _T, (T -> _T) -> _T -> _T.
-
-  Definition PredError {T} (P : T -> Prop) (m : Error T) : Prop :=
-    @m Prop P True.
-
-  Definition Error_bind {T U} (m : Error T) (k : T -> Error U) : Error U :=
-    fun _T good bad =>
-      @m _T (fun x => @k x _T good bad) bad.
-
-  Theorem Error_bind_sound
-  : forall {T U} P Q R m k,
-      PredError Q m ->
-      (forall x, PredError (fun z => Q x -> R x z) (k x)) ->
-      PredError P (@Error_bind T U m k).
-  Proof.
-    compute. intros.
-
-End with_error.
-*)
-
-Section with_nd.
-  Inductive lazy_choice (T : Type) : Type :=
-  | Done
-  | Choice : T -> (unit -> lazy_choice T) -> lazy_choice T.
-
-  Inductive PredChoice {T} (P : T -> Prop) : lazy_choice T -> Prop :=
-  | PredChoice_Done : PredChoice P (Done T)
-  | PredChoice_Choice : forall t rest,
-      P t ->
-      PredChoice P (rest tt) ->
-      PredChoice P (Choice t rest).
-
-  Fixpoint Choice_bind {T U} (m : lazy_choice T) (k : T -> lazy_choice U) {struct m} : lazy_choice U :=
-    match m with
-    | Done _ => Done _
-    | Choice a b =>
-      (fix iter (l : lazy_choice U) : lazy_choice U :=
-         match l with
-         | Done _ => Choice_bind (b tt) k
-         | Choice x xs => Choice x (fun x => iter (xs x))
-         end) (k a)
-    end.
-
-  Theorem Choice_bind_sound
-  : forall {T U} (P : T -> Prop) (Q : _ -> Prop) m k,
-      PredChoice P m ->
-      (forall x, PredChoice (fun y => P x -> Q y) (k x)) ->
-      PredChoice Q (@Choice_bind T U m k).
-  Proof.
-    compute. intros.
-    induction H.
-    { constructor. }
-    { specialize (H0 t).
-      induction H0; eauto.
-      { constructor; eauto. } }
-  Qed.
-
-End with_nd.
-
-
-(*******
-Section with_error.
-  Definition Error (T : Type) : Type := option T.
-
-  Definition PredError {T} (P : (T -> Prop) -> Prop -> Prop) (m : Error T) : Prop :=
-    match m with
-    | None => P (fun _ => False) True
-    | Some x => P (eq x) False
-    end.
-
-  Definition Error_bind {T U} (m : Error T) (k : T -> Error U) : Error U :=
-    match m with
-    | None => None
-    | Some x => k x
-    end.
-
-
-  Require Import Morphisms.
-
-
-  Definition LR {T} := ((@eq T ==> iff) ==> iff ==> iff)%signature.
-
-  Theorem Error_bind_sound
-  : forall {T U} (P : (T -> Prop) -> Prop -> Prop) (Q : _ -> _ -> Prop) m (k : T -> Error U)
-      (H:Proper LR P) (H' : Proper LR Q),
-      PredError P m ->
-      (forall x, PredError (fun kS kF => Q (fun y => (forall Z, P Z False -> Z x)-> kS y) kF) (k x)) ->
-      PredError (fun kS kF => Q kS kF \/ P (fun _ => False) kF) (@Error_bind T U m k).
-  Proof.
-    compute. intros.
-    destruct m.
-    { specialize (H1 t).
-      destruct (k t); auto.
-      { admit. }
-      { admit. } }
-    { clear H0. auto. }
-  Admitted.
-
-  Theorem Error_ret_sound {T} (v : T) : PredError (fun kP kF => (forall x, kP x -> x = v) /\ (kF -> False)) (Some v).
-  Proof.
-    compute. split; auto.
-  Qed.
-
-  Theorem Error_fail_sound {T} : PredError (fun kP kF => (forall x, kP x -> False) /\ kF) (@None T).
-  Proof.
-    compute. tauto.
-  Qed.
-
-  Theorem Proper_PredError_iff {T}
-  : Proper (((eq ==> iff) ==> iff ==> iff) ==> eq ==> iff)%signature (@PredError T).
-  Proof.
-    cbv beta iota zeta delta - [ iff ].
-    intros. subst.
-    destruct y0; try tauto.
-    eapply H. intros; subst; tauto. tauto.
-    eapply H; try tauto.
-  Qed.
-
-(*
-  Theorem Proper_PredError_impl {T} : Proper (((eq ==> iff) ==> Basics.impl) ==> eq ==> Basics.impl)%signature (@PredError T).
-  Proof.
-    cbv beta iota zeta delta - [ iff ].
-    intros. subst.
-    destruct y0; try tauto.
-    revert H1. eapply H.
-    intros. subst. tauto.
-  Qed.
-*)
-
-  Opaque PredError.
-
-  Goal PredError (fun kP kF => (forall x, kP x -> x = 3) /\ (kF -> False)) (Error_bind (Some 3) (@Some _)).
-  Proof.
-    eapply Proper_PredError_iff.
-    2: reflexivity.
-    2: eapply Error_bind_sound.
-    2: eapply Error_ret_sound.
-    Focus 2.
-    intros; simpl.
-    eapply Proper_PredError_iff.
-    2: reflexivity.
-    2: eapply Error_ret_sound.
-    red. red. intros.
-    instantiate (1:= fun kS kF => (forall x, kS x -> x = 3) /\ (kF -> False)). simpl.
-    split.
-    { intros. destruct H1.
-      Require Import Setoid.
-      red in H. rewrite <- H0. split; auto.
-      intros.
-      setoid_rewrite H0 in H1.
-      specialize (H1 x).
-
-  Qed.
-
-  Goal PredError (fun kP => kP 3) (Error_bind None (@Some _)).
-  Proof.
-    eapply Error_bind_sound.
-    eapply Error_fail_sound.
-    simpl.
-    intros.
-    eapply Proper_PredError_impl.
-    2: reflexivity.
-    2: eapply Error_ret_sound.
-    cbv beta iota zeta delta - [ iff ].
-    intros; subst. eapply H; eauto.
-  Qed.
-
-
-End with_error.
-****)
